<section xml:id="Sec_QuotientRule">
  <title>Quotient Rule</title>
  <introduction>
    <p>
      If we have a rule for differentiating products,
      we should have a rule for differentiating quotients as well,
      after all,
      quotients and products are basically the same thing.
      So let <m>Q(x)=\frac{f(x)}{g(x)}</m>,
      and ask, what is <m>Q'(x)</m>.
      So:
      <md>
        <mrow>Q(x)\amp =\amp \frac{f(x)}{g(x)}</mrow>
        <mrow>Q(x)g(x)\amp =\amp f(x),\ \text{ now we can differentiate both sides }</mrow>
        <mrow>\frac{d}{dx}[Q(x)g(x)]\amp =\amp f'(x),\ \text{ then by the product rule: }</mrow>
        <mrow>Q'(x)g(x)+Q(x)g'(x)\amp =\amp f'(x)</mrow>
        <mrow>Q'(x)g(x)\amp =\amp f'(x)-Q(x)g'(x),\ \text{then recall that  \(Q(x)=\frac{f(x)}{g(x)}\)}</mrow>
        <mrow>Q'(x)g(x)\amp =\amp f'(x)-\frac{f(x)g'(x)}{g(x)}</mrow>
        <mrow>Q'(x)g(x)\amp =\amp \frac{f'(x)g(x)-f(x)g'(x)}{g(x)}</mrow>
        <mrow>Q'(x)\amp =\amp \frac{f'(x)g(x)-f(x)g'(x)}{g(x)^2}</mrow>
      </md>
    </p>
    <p>
      So the <term> quotient rule</term>
      is <m>\frac{d}{dx}[\frac{f(x)}{g(x)}]=\frac{f'(x)g(x)-f(x)g'(x)}{g(x)^2}</m>.
    </p>
  </introduction>
  <subsection>
    <title>Examples</title>
    <p>
      So, consider the derivative of
      <m>f(x)=x^3(x+1)</m>, which can be computed:
      <md>
        <mrow>f'(x)\amp =\amp \frac{d}{dx}[x^3](x+1)+x^3\frac{d}{dx}[x+1]</mrow>
        <mrow>\amp =\amp 3x^2(x+1)+x^3(1)</mrow>
        <mrow>\amp =\amp 3x^3+3x^2+x^3</mrow>
        <mrow>\amp =\amp 4x^3+3x^2</mrow>
      </md>.
    </p>
    <p>
      Also note we could have computed this some other way:
      <md>
        <mrow>f(x)\amp =\amp x^3(x+1)=x^4+x^3</mrow>
        <mrow>f'(x)\amp =\amp 4x^3+3x^2</mrow>
      </md>.
    </p>
    <p>
      Similarly, the derivative of <m>g(x)=\frac{x}{x^2+1}</m>:
      <md>
        <mrow>g'(x)\amp =\amp \frac{(x^2+1)\frac{d}{dx}[x]-x\frac{d}{dx}[x^2+1]}{(x^2+1)^2}</mrow>
        <mrow>\amp =\amp \frac{(x^2+1)(1)-x(2x)}{(x^2+1)^2}</mrow>
        <mrow>\amp =\amp \frac{1-x^2}{(x^2+1)^2}</mrow>
      </md>
    </p>
  </subsection>
</section>