<section xml:id="Sec_PowerRule">
  <title>Power Rule</title>
  <introduction>
    <p>
      We may have noticed a pattern with derivatives.
      But to illustrate it explicitly:
      <ul>
        <li>
          <p>
            The derivative of <m>f(x)=x^0</m>,
            it's the derivative of the constant function <m>f(x)=1</m>,
            and since its a horizontal line,
            it never has any slope and <m>f'(x)=0</m>.
          </p>
        </li>
        <li>
          <p>
            The derivative of <m>f(x)=x^1</m>,
            it's the derivative of the line <m>f(x)=x</m> which always has slope 1, so <m>f'(x)=1</m>.
          </p>
        </li>
        <li>
          <p>
            The derivative of <m>f(x)=x^2</m> is:
            <md>
              <mrow>f(x)\amp =\amp \limit{h}{0}\frac{f(x+h)-f(x)}{h}</mrow>
              <mrow>\amp =\amp \limit{h}{0} \frac{(x+h)^2-x^2}{h}</mrow>
              <mrow>\amp =\amp \limit{h}{0} \frac{x^2+2xh+h^2-x^2}{h}</mrow>
              <mrow>\amp =\amp \limit{h}{0} \frac{(2x+h)h}{h}</mrow>
              <mrow>\amp =\amp \limit{h}{0} 2x+h=2x</mrow>
            </md>.
          </p>
        </li>
        <li>
          <p>
            The derivative of <m>f(x)=x^3</m> is:
            <md>
              <mrow>f(x)\amp =\amp \limit{h}{0}\frac{f(x+h)-f(x)}{h}</mrow>
              <mrow>\amp =\amp \limit{h}{0} \frac{(x+h)^3-x^3}{h}</mrow>
              <mrow>\amp =\amp \limit{h}{0} \frac{x^3+3x^2h+3xh^2+h^3-x^3}{h}</mrow>
              <mrow>\amp =\amp \limit{h}{0} \frac{(3x^2+3xh+h^2)h}{h}</mrow>
              <mrow>\amp =\amp \limit{h}{0} 3x^2+3xh+h^2=3x^2</mrow>
            </md>.
          </p>
        </li>
      </ul>
    </p>
    <p>
      To generalize this, we have a rule of differentiation called the
      <term> power rule</term> which goes:
      <m>\frac{d}{dx}[x^n]=nx^{n-1}</m>.
    </p>
    <p>
      To verify:
      <ul>
        <li>
          <p>
            <m>\frac{d}{dx}[x^0]=0x^{0-1}=0</m>.
          </p>
        </li>
        <li>
          <p>
            <m>\frac{d}{dx}[x^1]=1x^{1-1}=1</m>.
          </p>
        </li>
        <li>
          <p>
            <m>\frac{d}{dx}[x^2]=2x^{2-1}=2x</m>.
          </p>
        </li>
        <li>
          <p>
            <m>\frac{d}{dx}[x^3]=3x^{3-1}=3x^2</m>.
          </p>
        </li>
      </ul>
    </p>
    <p>
      What's fascinating is that this rule applies to <term> all</term>
      powers, not just integer powers.
    </p>
  </introduction>
  <subsection>
    <title>Examples</title>
    <p>
      We can combine these rules to find the derivatives of some basic functions.
      So consider the derivative of <m>f(x)=x^4-2x^2+7x-3</m>.
      It would be:
      <md>
        <mrow>f'(x)\amp =\amp \frac{d}{dx}[x^4-2x^2+7x-3]</mrow>
        <mrow>\amp =\amp \frac{d}{dx}[x^4-2x^2+7x^1-3x^0]</mrow>
        <mrow>\amp =\amp 4x^3-2(2x^1)+7(1x^0)-3(0x^{-1})</mrow>
        <mrow>\amp =\amp 12x^3-4x+7</mrow>
      </md>.
    </p>
    <p>
      Whereas the derivative of <m>g(x)=\sqrt{4x}+\frac{3}{x}-\frac{2}{x^2}</m> would be:
      <md>
        <mrow>g'(x)\amp =\amp \frac{d}{dx}[\sqrt{4x}+\frac{3}{x}-\frac{2}{x^2}]</mrow>
        <mrow>\amp =\amp \frac{d}{dx}[2x^{1/2}+3x^{-1}-2x^{-2}]</mrow>
        <mrow>\amp =\amp 2(1/2)x^{-1/2}+3(-1x^{-2})-2(2x^{-3})</mrow>
        <mrow>\amp =\amp x^{-1/2}-3x^{-2}+4x^{-3}</mrow>
        <mrow>\amp =\amp \frac{1}{\sqrt{x}}-\frac{3}{x^2}+\frac{4}{x^3}</mrow>
      </md>.
    </p>
  </subsection>
</section>