<section>
  <title>Product Rule</title>
  <p>
    Since the behavior of derivatives of sums behave so well,
    its tempting to believe that the derivatives of products would behave similarly well, that is,
    it may be reasonable to guess that <m>\frac{d}{dx}[f(x)g(x)]=f'(x)g'(x)</m>.
    To try to see if this is true, we should ask, is:
    <me>
      \frac{d}{dx}[x\cdot x]=\frac{d}{dx}[x]\frac{d}{dx}[x]?
    </me>
  </p>
  <p>
    Well on the left hand side <m>\frac{d}{dx}[x\cdot x]=\frac{d}{dx}[x^2]=2x</m>.
    On the right, <m>\frac{d}{dx}[x]\frac{d}{dx}[x]=1\cdot1=1</m>,
    so these are clearly not the same.
    What should it be?
  </p>
  <p>
    We do have a rule for products called the
    <term> product rule</term>
    and it states <m>\frac{d}{dx}[f(x)g(x)]=f'(x)g(x)+f(x)g'(x)</m>.
    To see why:
    <md>
      <mrow>\frac{d}{dx}[f(x)g(x)]\amp =\amp \limit{h}{0}\frac{f(x+h)g(x+h)-f(x)g(x)}{h},\ \text{ at this stage, I'm going to pull a clever trick and add by 0: }</mrow>
      <mrow>\amp =\amp \limit{h}{0}\frac{f(x+h)g(x+h)\textcolor{blue}{-f(x)g(x+h)+f(x)g(x+h)}-f(x)g(x)}{h}</mrow>
      <mrow>\amp =\amp \limit{h}{0}\frac{f(x+h)g(x+h)-f(x)g(x+h)}{h}+\limit{h}{0}\frac{f(x)g(x+h)-f(x)g(x)}{h}</mrow>
      <mrow>\amp =\amp \limit{h}{0}\frac{f(x+h)-f(x)}{h}g(x+h)+\limit{h}{0}f(x)\frac{g(x+h)-g(x)}{h}</mrow>
      <mrow>\amp =\amp f'(x)g(x)+f(x)g'(x)</mrow>
    </md>.
  </p>
</section>